wip for proofs from spec1 to spec2

proofs/compiler/spec1_spec2.v
@@ -21,7 +21,9 @@ End E.
 Definition cond_env_rec (e : pexpr) :=
 if use_mem e then None else Some e.
 
-Definition cond_env := option pexpr.
+(* expression defining the boolean condition and Sv.t defining the 
+   free variables present in e *)
+Definition cond_env := option (pexpr * Sv.t).
 
 Definition cond_env_empty : cond_env := None.
 
@@ -31,22 +33,27 @@ Definition env := (cond_env * var_env)%type.
 
 Definition empty_env := (cond_env_empty, Sv.empty).
 
-Definition is_some (e : cond_env) := 
-match e with 
-| Some e => true 
-| None => false
+Definition get_fv (env : cond_env) : Sv.t :=
+match env with 
+| Some e => e.2
+| None => Sv.empty
 end.
 
-Definition is_some_mem_op_free (E : cond_env) := 
-match E with 
-| Some e' => let r := cond_env_rec e' in
-             (*let re := eq_expr e' e in *)
-             if is_some r then true else false
-| None => false
-end.
+Inductive wf_env (envi : env) : Prop :=
+| wf_cond_env : forall e fv msf,
+                envi = (Some (e, fv), msf)  ->
+                fv = read_e e ->
+                use_mem e = false ->
+                wf_env envi
+| wf_none_env : forall msf,
+                envi = (None, msf) ->
+                wf_env envi.
  
-(* FIX ME *)
-Definition update_cond_env (E : cond_env) : cond_env := E.
+Definition update_cond_env (X: Sv.t) (E : cond_env) : cond_env :=
+match E with 
+| Some (e, fv) => if Sv.subset X fv then None else E
+| None => None
+end.
 
 Section ASM_OP.
 
@@ -103,74 +110,66 @@ Fixpoint ir_spec1_to_spec2 envi ii (ir: @instr_r asm_op_spec1 asmOp_spec1) {stru
 : cexec (env * seq (@instr asm_op_spec2 asmOp_spec2)) := 
 match ir with 
 | Cassgn x tag ty e => ok (envi, [:: MkI ii (@Cassgn asm_op_spec2 asmOp_spec2 x tag ty e)])
-| Copn xs tag o es => let cr := [:: MkI ii (@Copn asm_op_spec2 asmOp_spec2 xs tag 
-                                            ((sopn_spec1_to_spec2 o)) es)] in
-                      match o with 
-                      | Ocopy _ _ => ok (envi, cr) 
-                      | Onop => ok (envi, cr) 
-                      | Omulu _ => ok (envi, cr)
-                      | Oaddcarry _ => ok (envi, cr)
-                      | Osubcarry _ => ok (envi, cr)
-                      (* xs := init_msf 
-                         X = xs U X 
-                         E = .... *)
-                      | sopn.Oasm asm_op_spec1.Oinit_msf =>
-                        match es with 
-                        | [::] => let cenv := update_cond_env envi.1 in 
-                                  let venv := vrvs_rec envi.2 xs in  
-                                  ok ((cenv, venv), cr)
-                        | _ => Error (spec_transform_error "Too many arguments")
-                        end 
-                      (* xs := set_msf (e, y) 
-                         here y represents the msf flag and e is the boolean 
-                         X = xs U X (E is Some e and y in X) 
-                         X = X (y not in X) *)
-                      | sopn.Oasm asm_op_spec1.Oset_msf =>
-                        match es with 
-                        | [:: e ; y] => 
-                          let cenv := update_cond_env envi.1 in
-                          let r1 := is_some_mem_op_free envi.1 in 
-                          let rs := read_e_rec Sv.empty y in
-                          let r2 := disjoint rs envi.2 in
-                          if r1 && negb r2
-                          then ok ((cenv, vrvs_rec envi.2 xs), cr)
-                          else ok ((cenv, envi.2), cr)
-                        | _ =>  Error (spec_transform_error "Too many arguments")
-                         end 
-                      (* xs := protect (e, y)
-                         should fail if y is not in X *)
-                      | sopn.Oasm (asm_op_spec1.Oprotect w) => 
-                        match es with 
-                        | [:: e; y] =>
-                          let cenv := update_cond_env envi.1 in 
-                          let rs := read_e_rec Sv.empty y in 
-                          let r := disjoint rs envi.2 in 
-                          if r 
-                          then Error (spec_transform_error "Msf variable not present")
-                          else ok ((cenv, envi.2), cr)
-                        | _ => Error (spec_transform_error "Too many arguments")
-                        end
-                      (* xs := mov_msf(y) 
-                         if y is present in msf set then xs U X else X *)
-                      | sopn.Oasm asm_op_spec1.Omov_msf => 
-                        match es with
-                        | [:: y] => 
-                          let rs := read_e_rec Sv.empty y in 
-                          let r := disjoint rs envi.2 in
-                          if r 
-                          then ok ((update_cond_env envi.1, envi.2), cr)
-                          else ok ((update_cond_env envi.1, vrvs_rec envi.2 xs), cr)
-                        | _ => Error (spec_transform_error "Too many arguments")
-                        end
-                      | sopn.Oasm o => 
-                        ok (envi, cr) 
-                      end
+| Copn xs tag o es => 
+  let cr := [:: MkI ii (@Copn asm_op_spec2 asmOp_spec2 xs tag ((sopn_spec1_to_spec2 o)) es)] in
+  match o with 
+  | Ocopy _ _ | Onop | Omulu _ | Oaddcarry _ | Osubcarry _ => ok (envi, cr)
+    (* xs := init_msf 
+       X = xs U X 
+       E = update E based on whether X is present in E or not *)
+  | sopn.Oasm asm_op_spec1.Oinit_msf =>
+    match es with 
+    | [::] => let cenv := update_cond_env envi.2 envi.1 in 
+              let venv := vrvs_rec envi.2 xs in  
+              ok ((cenv, venv), cr)
+    | _ => Error (spec_transform_error "Too many arguments")
+    end 
+    (* xs := set_msf (e, y) 
+       here y represents the msf flag and e is the boolean 
+       X = xs U X (E is Some e and y in X) 
+       X = X (y not in X) *)
+  | sopn.Oasm asm_op_spec1.Oset_msf =>
+    match es with 
+    | [:: e ; y] => let cenv := update_cond_env envi.2 envi.1 in
+                    let rs := read_e_rec Sv.empty y in
+                    let r2 := disjoint rs envi.2 in
+                    if negb r2
+                    then ok ((cenv, vrvs_rec envi.2 xs), cr)
+                    else ok ((cenv, envi.2), cr)
+    | _ =>  Error (spec_transform_error "Too many arguments")
+   end 
+   (* xs := protect (e, y)
+      should fail if y is not in X *)
+  | sopn.Oasm (asm_op_spec1.Oprotect w) => 
+    match es with 
+    | [:: e; y] => let cenv := update_cond_env envi.2 envi.1 in 
+                   let rs := read_e_rec Sv.empty y in 
+                   let r := disjoint rs envi.2 in 
+                   if r 
+                   then Error (spec_transform_error "Msf variable not present")
+                   else ok ((cenv, envi.2), cr)
+    | _ => Error (spec_transform_error "Too many arguments")
+    end
+   (* xs := mov_msf(y) 
+      if y is present in msf set then xs U X else X *)
+  | sopn.Oasm asm_op_spec1.Omov_msf => 
+    match es with
+    | [:: y] => let rs := read_e_rec Sv.empty y in 
+                let r := disjoint rs envi.2 in
+                if r 
+                then ok ((update_cond_env envi.2 envi.1, envi.2), cr)
+                else ok ((update_cond_env envi.2 envi.1, vrvs_rec envi.2 xs), cr)
+    | _ => Error (spec_transform_error "Too many arguments")
+    end
+  | sopn.Oasm o => ok (envi, cr) 
+  end
  (* FIX ME *)                   
 | Csyscall xs o es => ok (envi, [:: MkI ii (@Csyscall asm_op_spec2 asmOp_spec2 xs o es)])
 (* FIX ME *)
-| Cif b c1 c2 => Let rc1 := (c_spec1_to_spec2 i_spec1_to_spec2 (Some b, envi.2) c1) in 
-                 Let rc2 := (c_spec1_to_spec2 i_spec1_to_spec2 (Some b, envi.2) c2) in 
-                 ok ((None, Sv.inter rc1.1.2 rc2.1.2), [:: MkI ii (@Cif asm_op_spec2 asmOp_spec2 b rc1.2 rc2.2)])
+| Cif b c1 c2 => 
+  Let rc1 := (c_spec1_to_spec2 i_spec1_to_spec2 (Some (b, get_fv envi.1), envi.2) c1) in 
+  Let rc2 := (c_spec1_to_spec2 i_spec1_to_spec2 (Some ((enot b), get_fv envi.1), envi.2) c2) in 
+  ok ((update_cond_env envi.2 envi.1, Sv.inter rc1.1.2 rc2.1.2), [:: MkI ii (@Cif asm_op_spec2 asmOp_spec2 b rc1.2 rc2.2)])
 | Cfor x (dir, e1, e2) c => Let cr := c_spec1_to_spec2 i_spec1_to_spec2 envi c in 
                             ok (cr.1, [:: MkI ii (@Cfor asm_op_spec2 asmOp_spec2 x (dir, e1, e2) cr.2)])
 | Cwhile a c e c' => (*let c := (c_spec1_to_spec2 i_spec1_to_spec2 c) in 
@@ -212,8 +211,6 @@ End Section.
 
 Section PROOF.
 
-Search concl : semCallParams.
-
 Context
   {syscall_state asm_op : Type}
   `{asmop : asmOp}
@@ -224,7 +221,9 @@ Context
 Existing Instance progUnit.
 
 Variable (ev:extra_val_t).
-Variable (p: @prog asm_op_spec1 asmOp_spec1 _ _).
+(*Variable (p: @prog asm_op_spec1 asmOp_spec1 _ _).*)
+
+Variable (p: @prog asm_op_spec1  (@asmOp_of_spp (@asm_op_spec1 asm_op0 asmop) _ _) _ _).
 
 (*Context {T:eqType} {pT:progT T} `{sCP: semCallParams}.
 Variable (ev:extra_val_t).
@@ -237,28 +236,158 @@ cexec (env * @fundef asm_op_spec2 asmOp_spec2 _ _)) ->
 @prog asm_op_spec1 asmOp_spec1 _ _ -> 
 @prog asm_op_spec2 asmOp_spec2 _ _.
 
+Definition estate_spec1_spec2 (s1 : @estate (@asm_op_spec1 asm_op0 asmop) syscall_state
+                  (@spp_of_asm_op_spec1 asm_op0 asmop pd syscall_state fcp sc_sem)) :
+@estate (@asm_op_spec2 asm_op0 asmop) syscall_state
+                  (@spp_of_asm_op_spec2 asm_op0 asmop pd syscall_state fcp sc_sem) :=
+match s1 with 
+| Estate ss m f => @Estate (@asm_op_spec2 asm_op0 asmop) syscall_state
+                   (@spp_of_asm_op_spec2 asm_op0 asmop pd syscall_state fcp sc_sem) ss m f
+end. 
+
 Let p' := prog_spec1_to_spec2 map_spec1_to_spec2 p.
 
-Let Pi_r s1 ii (i: @instr_r asm_op_spec1 asmOp_spec1) (envi : env) :=
+Let Pi_r s1 (i: @instr_r asm_op_spec1 asmOp_spec1) s2 :=
+forall ii (envi : env), 
+wf_env envi ->
 match (ir_spec1_to_spec2 envi ii i) with
- | Ok (envi', c') => exists s2, sem p' ev s1 c' s2
+ | Ok (envi', c') => sem p' ev (estate_spec1_spec2 s1) c' (estate_spec1_spec2 s2) /\ wf_env envi'
  | _ => True
 end.
 
-Let Pi s1 i (envi : env) :=
+Let Pi s1 i s2 :=
+forall (envi : env),
+wf_env envi ->
 match (i_spec1_to_spec2 envi i) with
- | Ok (envi', c') => exists s2, sem p' ev s1 c' s2
+ | Ok (envi', c') => sem p' ev (estate_spec1_spec2 s1) c' (estate_spec1_spec2 s2) /\ wf_env envi'
  | _ => True
 end.
 
-Let Pc s1 c (envi : env) :=
+Let Pc s1 c s2 :=
+forall (envi : env),
+wf_env envi ->
 match (c_spec1_to_spec2 (i_spec1_to_spec2) envi c) with
- | Ok (envi', c') => exists s2, sem p' ev s1 c' s2
+ | Ok (envi', c') => sem p' ev (estate_spec1_spec2 s1) c' (estate_spec1_spec2 s2) /\ wf_env envi'
  | _ => True
 end.
 
-Let Pfor s1 c (envi : env) vs i :=
+Let Pfor i vs s1 c s2 :=
+forall (envi : env),
+wf_env envi ->
 match (c_spec1_to_spec2 (i_spec1_to_spec2) envi c) with
- | Ok (envi', c') => exists s2, sem_for p' ev i vs s1 c' s2
+ | Ok (envi', c') => sem_for p' ev i vs (estate_spec1_spec2 s1) c' (estate_spec1_spec2 s2) /\ wf_env envi'
  | _ => True
 end.
+
+(*Set Printing Implicit.
+Set Printing All.
+About sem_Ind_nil. About estate. Print estate. Print sem_Ind_nil.
+Print Instances SemPexprParams. 
+Print Pc.
+Print Estate.*)
+
+Lemma eq_globs : p_globs p = p_globs p'.
+Proof.
+rewrite /p' /=. case: p=> /=. 
+move=> pf pg pe /=. rewrite /prog_spec1_to_spec2 /= /fun_spec1_to_spec2 /=. 
+Admitted.
+
+Lemma Hskip : sem_Ind_nil Pc.
+Proof.
+move=> s1 envi hwf /=. split=> //=.
+rewrite /estate_spec1_spec2. case: s1=> //=. 
+by constructor.
+Qed.
+
+Lemma Hcons : sem_Ind_cons p ev Pc Pi.
+Admitted.
+
+Lemma HmkI : sem_Ind_mkI p ev Pi_r Pi.
+Admitted.
+
+Lemma Hassgn : sem_Ind_assgn p Pi_r.
+Proof.
+move=> s1 s2 x tag ty e v v' he ht hw. rewrite /Pi_r /=.
+move=> ii envi hwf /=.
+have heg := eq_globs. split=> //=.
++ rewrite /estate_spec1_spec2 /=. case: s1 he ht hw=> //= ss m f he ht hw. 
+  case: s2 hw=> //= ss' m' f' hw. econstructor. 
+  + econstructor. econstructor.
+    + rewrite -heg /=.  admit.
+    + by apply ht.
+    rewrite -heg /=. admit.
+  by constructor.
+Admitted.
+
+Lemma Hopn : sem_Ind_opn p Pi_r.
+Proof.
+move=> s1 s2 t [].
+(* Ocopy *)
++ move=> w pos xs es /= hop. rewrite /Pi_r /=. have heg := eq_globs.
+  move=> ii envi hwf /=. split=> //=.
+  rewrite /estate_spec1_spec2 /=. case: s1 hop=> //= ss m vm hop.
+  case: s2 hop=>//= ss' m' vm' hop'. econstructor.
+  econstructor. + econstructor. rewrite -heg /=. admit.
+  by constructor.
+(* Onop *)
++ move=> xs es hop. rewrite /Pi_r /=. have heg := eq_globs.
+  move=> ii envi hwf /=. split=> //=. econstructor. 
+  + econstructor. econstructor. rewrite -heg. admit.
+  by constructor.
+(* Omul *)
++ admit.
+(* Oaddcarry *)
++ admit.
+(* Osubcarry *)
++ admit.
+move=> [].
+(* protect *)
++ admit.
+(* set_msf *)
++ admit.
+(* init_msf *)
++ move=> xs [] //= hop. rewrite /Pi_r /= /estate_spec1_spec2 /=. have heg := eq_globs.
+  case: s1 hop=> //=. case: s2=> //=.
+  move=> ss' m' vm' ss m vm /= hop ii envi hwf /=.
+  split=> //=.
+  + econstructor.
+    + econstructor. econstructor. rewrite -heg. Set Printing Implicit.  admit.
+    by constructor.
+  case: hwf=> //=.
+  (* some *)
+  + move=> e fv msf -> -> hmem /=. case: ifP=> //=.
+    + move=> hsub. by apply wf_none_env with (vrvs_rec msf xs).
+    move=> hsub. by apply wf_cond_env with e (read_e e) (vrvs_rec msf xs).
+  (* none *)
+  move=> msf -> /=. by apply wf_none_env with (vrvs_rec msf xs).
+(* mov_msf *)
++ move=> xs es hop. rewrite /Pi_r /ir_spec1_to_spec2 /estate_spec1_spec2 /=. have heg := eq_globs.
+  case: s1 hop=> //=. case: s2=> //=. move=> ss' m' vm' ss m vm /= hop.
+  case: es hop=> //= e es. case: es=> //= hop ii envi hwf.
+  case: ifP=> //=.
+  (* e not present in X ==> X = X*)
+  + move=> hdisj. split=> //=.
+    + econstructor.
+      + econstructor. econstructor.
+  
+Admitted.
+
+Lemma Hif_true : sem_Ind_if_true p ev Pc Pi_r.
+Admitted.
+
+Lemma Hif_false : sem_Ind_if_false p ev Pc Pi_r.
+Admitted.
+
+Lemma Hwhile_true : sem_Ind_while_true p ev Pc Pi_r.
+Admitted.
+
+Lemma Hwhile_false : sem_Ind_while_false p ev Pc Pi_r.
+Admitted.
+
+Lemma Hfor : sem_Ind_for p ev Pi_r Pfor.
+Admitted.
+
+
+
+
+
